---
title: Converging series
---

## Lemma
Let \\( 0 < x < 1\\), the sum \\(1 + x + x^2 + x^3 + x^4 + \\cdots\\) converges.

## Proof

\\[
\\lim\_{n \\to \\infty} x^n = 0.
\\]

## Theorem

Let \\( 0 < x < 1\\),
\\[
1 + x + x^2 + x^3 + x^4 + \\cdots = \\frac{1}{1-x}.
\\]

## Proof

\\begin{align}
1 + x + x^2 + x^3 + x^4 + \\cdots &= \\frac{1}{1-x} \\\\\\\\
(1 - x)(1 + x + x^2 + x^3 + x^4 + \\cdots) &= 1 \\\\\\\\
1 + x + x^2 + x^3 + x^4 + \\cdots - (x + x^2 + x^3 + x^4 + \\cdots) &= 1.
\\end{align}
